modify tidRA and fix SchIAproof

scheduler/SchA.v
@@ -1,7 +1,7 @@
 Require Import CRIS.
 Require Import SchHeader SchI.
 Require Import CallFilter.
-From iris Require Import frac_auth.
+From iris Require Import frac_auth dfrac_agree.
 
 Set Implicit Arguments.
 
@@ -16,8 +16,10 @@ Section SchRA.
   Definition fragreeUR := optionUR (prodR fracR (agreeR thst)).
   Definition threadsF := nat -d> fragreeUR.
   Definition threadsRA := authUR threadsF.
-
-  Definition tidRA := nat -d> optionUR fracR.
+  
+  Definition tidF := nat -d> optionUR fracR.
+  Definition tidA := optionUR (dfrac_agreeR (optionO natO)).
+  Definition tidRA := prodR tidF tidA.
 
   Class schG `{!crisG Γ Σ α β τ _S _I} := {
       sch_inG_tid :: inG tidRA Γ;
@@ -70,20 +72,25 @@ Module SchAS. Section SchAS.
     Seal.sealing "SchA" (own base_γ (token_one_r tid st)).
 
   (** tid **)
-  Definition tid_admin_r (otid: option nat) : tidRA :=
+  Definition tid_admin_r (otid: option nat) : tidF :=
     match otid with
     | Some tid =>
         (λ t, if t =? tid then ε else Some 1)
     | None =>
         (λ t, Some 1)
     end.
-  Definition tid_user_r (q: Qp) (tid: nat) : tidRA :=
+  Definition tid_user_r (q: Qp) (tid: nat) : tidF :=
     (λ t, if t =? tid then Some q else ε).
 
+  Definition tid_frag_r (q: Qp) (otid: option nat) : tidA := Some (to_frac_agree q otid).
+
   Definition tid_admin (otid: option nat) : iProp Σ :=
-    Seal.sealing "SchA" (own base_γ (tid_admin_r otid)).
+    Seal.sealing "SchA" (own base_γ ((tid_admin_r otid, match otid with
+                                                        | Some tid => None
+                                                        | None => tid_frag_r 1 None
+                                                        end): tidRA)).
   Definition tid_user (q: Qp) (tid: nat) : iProp Σ :=
-    Seal.sealing "SchA" (own base_γ (tid_user_r q tid)).
+    Seal.sealing "SchA" (own base_γ ((tid_user_r q tid, tid_frag_r q (Some tid)): tidRA)).
 
   (** initial resource *)
   Definition ir_threadsRA : DRA_mk threadsRA := 
@@ -105,8 +112,8 @@ Module SchAS. Section SchAS.
   Qed.
 
   Definition ir_tidRA : DRA_mk tidRA :=
-    tid_admin_r None.
-  Lemma ir_tidRA_valid : ✓ (ir_tidRA). intro i; ss. Qed.
+    (tid_admin_r None, tid_frag_r 1 None).
+  Lemma ir_tidRA_valid : ✓ (ir_tidRA). econs; ss. Qed.
 
   Definition ir_schΓ : schΓ :=
     *[Some ir_tidRA].
@@ -116,9 +123,8 @@ Module SchAS. Section SchAS.
 
   Definition init_threads : iProp Σ := 
     Seal.sealing "SchA" (own base_γ ir_threadsRA).
-
-  Definition init_tid_r : tidRA := tid_admin_r (Some 0).
-  Definition init_tid : iProp Σ := Seal.sealing "SchA" (own base_γ init_tid_r)%I.
+  Definition init_tid : iProp Σ :=
+    Seal.sealing "SchA" (own base_γ (tid_admin_r (Some 0), None))%I.
 
   Section RA.
 
@@ -201,7 +207,8 @@ Module SchAS. Section SchAS.
     Proof using.
       rewrite /tid_admin /tid_user. unseal "SchA".
       iIntros "[A U]". iCombine "A U" gives %wf.
-      rewrite /tid_admin_r /tid_user_r in wf.
+      rewrite /tid_admin_r /tid_user_r /tid_frag_r in wf.
+      rewrite -pair_op pair_valid in wf; des; ss.
       specialize (wf t). rewrite discrete_fun_lookup_op in wf.
       rewrite Nat.eqb_refl -Some_op frac_op in wf. exfalso.
       apply (proj1 (Some_valid _)), (proj1 (frac_valid _)) in wf.
@@ -213,7 +220,8 @@ Module SchAS. Section SchAS.
     Proof using.
       rewrite /tid_admin /tid_user. unseal "SchA".
       iIntros "[F U]". iCombine "F U" gives %wf.
-      rewrite /tid_admin_r /tid_user_r in wf.
+      rewrite /tid_admin_r /tid_user_r /tid_frag_r in wf.
+      rewrite -pair_op pair_valid in wf; des; ss.
       specialize (wf t1). rewrite discrete_fun_lookup_op in wf.
       rewrite Nat.eqb_refl in wf.
       des_ifs.
@@ -224,29 +232,46 @@ Module SchAS. Section SchAS.
     Qed.
 
     Lemma tid_admin_none_split_r t :
-      (tid_admin_r (Some t): tidRA) ⋅ (tid_user_r 1 t: tidRA) = (tid_admin_r None: tidRA).
+      (tid_admin_r (Some t): tidF) ⋅ (tid_user_r 1 t: tidF) = (tid_admin_r None: tidF).
     Proof using.
       rewrite /tid_admin_r /tid_user_r. extensionalities x.
       rewrite !discrete_fun_lookup_op. des_ifs.
     Qed.
 
+    Lemma tid_frag_update_r ot0 ot1 :
+      tid_frag_r 1 ot0 ~~> tid_frag_r 1 ot1.
+    Proof using.
+      rewrite /tid_frag_r.
+      eapply option_update, cmra_update_exclusive; ss.
+    Qed.
+
     Lemma tid_admin_some_user_merge t :
-      tid_admin (Some t) ∗ tid_user 1 t ⊢ tid_admin None.
+      tid_admin (Some t) ∗ tid_user 1 t ⊢ |==> tid_admin None.
     Proof using.
       iIntros "[A U]".
       iPoseProof (tid_admin_some_user with "[A U]") as "%"; iFrame. des.
       rewrite /tid_admin /tid_user. unseal "SchA".
       iCombine "A U" as "AU".
       rewrite tid_admin_none_split_r; eauto.
+      iPoseProof (own_update with "AU") as ">AU".
+      { instantiate (1:=(tid_admin_r None, _)). eapply prod_update; s; [refl|].
+        rewrite left_id. eapply (tid_frag_update_r _ None). }
+      iFrame; eauto.
     Qed.
 
     Lemma tid_admin_none_split t :
-      tid_admin None ⊢ tid_admin (Some t) ∗ tid_user 1 t.
+      tid_admin None ⊢ |==> tid_admin (Some t) ∗ tid_user 1 t.
     Proof using.
       iIntros "N".
       rewrite /tid_admin /tid_user. unseal "SchA".
       rewrite -(tid_admin_none_split_r t); eauto.
-      iDestruct "N" as "[A U]". iFrame.
+      iPoseProof (own_update with "N") as ">N".
+      { instantiate (1 := (tid_admin_r (Some t) ⋅ tid_user_r 1 t, _)).
+        eapply prod_update; s; [refl|].
+        eapply (tid_frag_update_r _ (Some t)). }
+      replace (tid_admin_r (Some t) ⋅ tid_user_r 1 t, tid_frag_r 1 (Some t))
+        with ((tid_admin_r (Some t), None) ⋅ (tid_user_r 1 t, tid_frag_r 1 (Some t))) by ss.
+      iDestruct "N" as "[A U]". iFrame; eauto.
     Qed.
 
     Lemma tid_user_shrink q0 q tid
@@ -254,15 +279,23 @@ Module SchAS. Section SchAS.
       :
       tid_user q0 tid ⊢ tid_user q tid.
     Proof.
-      rewrite /tid_user /tid_user_r. unseal "SchA".
+      rewrite /tid_user /tid_user_r /tid_frag_r. unseal "SchA".
       eapply own_mono.
       destruct (q0 - q) eqn: E.
-      - exists (λ t : nat, if t =? tid then Some q1 else ε).
-        ii. rewrite discrete_fun_lookup_op. des_ifs.
-        apply Qp.sub_Some in E. subst. et.
-      - eapply Qp.sub_None in E. exists ε. rewrite right_id.
-        ii. des_ifs. eapply Qp.le_lteq in LE. eapply Qp.le_ngt in E.
-        des; subst; ss.
+      - exists (λ t : nat, if t =? tid then Some q1 else ε, Some (to_frac_agree q1 (Some tid))).
+        split; ss.
+        + ii. rewrite discrete_fun_lookup_op. des_ifs.
+          apply Qp.sub_Some in E. subst. et.
+        + rewrite -Some_op /to_frac_agree /to_dfrac_agree. f_equiv.
+          rewrite -pair_op agree_idemp. f_equiv.
+          rewrite dfrac_op_own. f_equiv.
+          eapply Qp.sub_Some; eauto.
+      - eapply Qp.sub_None in E. exists (ε, ε). rewrite -pair_op !right_id.
+        split; ss.
+        + ii. des_ifs. eapply Qp.le_lteq in LE. eapply Qp.le_ngt in E.
+          des; subst; ss.
+        + repeat f_equiv. eapply Qp.le_lteq in LE. eapply Qp.le_ngt in E.
+          des; subst; ss.
     Qed.
     
     Lemma tid_user_merge (q0 q1: Qp) tid
@@ -270,8 +303,11 @@ Module SchAS. Section SchAS.
       tid_user q0 tid ∗ tid_user q1 tid ⊢ tid_user (q0+q1) tid.
     Proof.
       rewrite /tid_user /tid_user_r. unseal "SchA".
-      rewrite -own_op. eapply own_mono. exists ε. rewrite right_id.
-      ii. rewrite discrete_fun_lookup_op. des_ifs.
+      rewrite -own_op. eapply own_mono. exists (ε, ε). rewrite -!pair_op !right_id.
+      split; ss.
+      - ii. rewrite discrete_fun_lookup_op. des_ifs.
+      - rewrite /tid_frag_r -Some_op /to_frac_agree /to_dfrac_agree.
+        f_equiv. rewrite -pair_op agree_idemp //.
     Qed.
 
     Lemma tid_user_split (q0 q1: Qp) tid
@@ -279,8 +315,11 @@ Module SchAS. Section SchAS.
       tid_user (q0+q1) tid ⊢ tid_user q0 tid ∗ tid_user q1 tid.
     Proof.
       rewrite /tid_user /tid_user_r. unseal "SchA".
-      rewrite -own_op. eapply own_mono. exists ε. rewrite right_id.
-      ii. rewrite discrete_fun_lookup_op. des_ifs.
+      rewrite -own_op. eapply own_mono. exists (ε, ε). rewrite -!pair_op !right_id.
+      split; ss.
+      - ii. rewrite discrete_fun_lookup_op. des_ifs.
+      - rewrite /tid_frag_r -Some_op /to_frac_agree /to_dfrac_agree.
+        f_equiv. rewrite -pair_op agree_idemp //.
     Qed.
 
     (* need to update the definition [tid_user] *)
@@ -288,7 +327,14 @@ Module SchAS. Section SchAS.
       :
       tid_user q0 tid0 ∗ tid_user q1 tid1 ⊢ ⌜tid0 = tid1⌝.
     Proof.
-    Admitted.
+      rewrite /tid_user /tid_user_r /tid_frag_r. unseal "SchA".
+      iIntros "[U U0]". iCombine "U U0" gives %wf.
+      rewrite -pair_op in wf. destruct wf as [wf0 wf]; ss.
+      rewrite -Some_op Some_valid in wf.
+      rewrite /to_frac_agree /to_dfrac_agree -pair_op in wf.
+      destruct wf as [wf1 wf]; ss.
+      rewrite to_agree_op_valid in wf. inv wf. eauto.
+    Qed.
     
   End RA.
 
